theories/program_logic/ectx_lifting.v
@@ -13,17 +13,6 @@ Implicit Types v : val.
 Implicit Types e : expr.
 Hint Resolve head_prim_reducible head_reducible_prim_step.
 Hint Resolve (reducible_not_val _ inhabitant).
-
-Definition head_progressive (e : expr) (σ : state) :=
-  is_Some(to_val e) ∨ ∃ K e', e = fill K e' ∧ head_reducible e' σ.
-
-Lemma progressive_head_progressive e σ :
-  progressive e σ → head_progressive e σ.
-Proof.
-  case=>[?|Hred]; first by left.
-  right. move: Hred=> [] e' [] σ' [] efs [] K e1' e2' EQ EQ' Hstep. subst.
-  exists K, e1'. split; first done. by exists e2', σ', efs.
-Qed.
 Hint Resolve progressive_head_progressive.
 
 Lemma wp_ectx_bind {p E e} K Φ :
@@ -42,25 +31,6 @@ Lemma wp_lift_head_step {p E Φ} e1 :
     ⌜head_reducible e1 σ1⌝ ∗
     ▷ ∀ e2 σ2 efs, ⌜head_step e1 σ1 e2 σ2 efs⌝ ={∅,E}=∗
       state_interp σ2 ∗ WP e2 @ p; E {{ Φ }} ∗ [∗ list] ef ∈ efs, WP ef @ p; ⊤ {{ _, True }})
-  ⊢ WP e1 @ p; E {{ Φ }}.
-Proof.
-  iIntros (?) "H". iApply wp_lift_step=>//. iIntros (σ1) "Hσ".
-  iMod ("H" with "Hσ") as "[% H]"; iModIntro.
-  iSplit; first by destruct p; eauto. iNext. iIntros (e2 σ2 efs) "%".
-  iApply "H"; eauto.
-Qed.
-
-(*
-  PDS: Discard. It's confusing. In practice, we just need rules
-  like wp_lift_head_{step,stuck}.
-*)
-Lemma wp_strong_lift_head_step p E Φ e1 :
-  to_val e1 = None →
-  (∀ σ1, state_interp σ1 ={E,∅}=∗
-    ⌜if p then head_reducible e1 σ1 else True⌝ ∗
-    ▷ ∀ e2 σ2 efs, ⌜prim_step e1 σ1 e2 σ2 efs⌝ ={∅,E}=∗
-      state_interp σ2 ∗ WP e2 @ p; E {{ Φ }}
-      ∗ [∗ list] ef ∈ efs, WP ef @ p; ⊤ {{ _, True }})
   ⊢ WP e1 @ p; E {{ Φ }}.
 Proof.
   iIntros (?) "H". iApply wp_lift_step=>//. iIntros (σ1) "Hσ".
@@ -91,18 +61,6 @@ Proof using Hinh.
   iIntros (????). iApply "H"; eauto.
 Qed.
 
-(* PDS: Discard. *)
-Lemma wp_strong_lift_pure_head_step p E Φ e1 :
-  to_val e1 = None →
-  (∀ σ1, if p then head_reducible e1 σ1 else True) →
-  (∀ σ1 e2 σ2 efs, prim_step e1 σ1 e2 σ2 efs → σ1 = σ2) →
-  (▷ ∀ e2 efs σ, ⌜prim_step e1 σ e2 σ efs⌝ →
-    WP e2 @ p; E {{ Φ }} ∗ [∗ list] ef ∈ efs, WP ef @ p; ⊤ {{ _, True }})
-  ⊢ WP e1 @ p; E {{ Φ }}.
-Proof using Hinh.
-  iIntros (???) "H". iApply wp_lift_pure_step; eauto. by destruct p; auto.
-Qed.
-
 Lemma wp_lift_pure_head_stuck E Φ e :
   to_val e = None →
   (∀ K e1 σ1 e2 σ2 efs, e = fill K e1 → ¬ head_step e1 σ1 e2 σ2 efs) →
@@ -114,64 +72,33 @@ Proof using Hinh.
   move=>[] K [] e1 [] Hfill [] e2 [] σ2 [] efs /= Hstep. exact: Hnstep.
 Qed.
 
-Lemma wp_lift_atomic_head_step {E Φ} e1 :
+Lemma wp_lift_atomic_head_step {p E Φ} e1 :
   to_val e1 = None →
   (∀ σ1, state_interp σ1 ={E}=∗
     ⌜head_reducible e1 σ1⌝ ∗
     ▷ ∀ e2 σ2 efs, ⌜head_step e1 σ1 e2 σ2 efs⌝ ={E}=∗
       state_interp σ2 ∗
-      default False (to_val e2) Φ ∗ [∗ list] ef ∈ efs, WP ef {{ _, True }})
-  ⊢ WP e1 @ E {{ Φ }}.
-Proof.
-  iIntros (?) "H". iApply wp_lift_atomic_step; eauto.
-  iIntros (σ1) "Hσ1". iMod ("H" $! σ1 with "Hσ1") as "[% H]"; iModIntro.
-  iSplit; first by eauto. iNext. iIntros (e2 σ2 efs) "%". iApply "H"; auto.
-Qed.
-
-(* PDS: Discard. *)
-Lemma wp_strong_lift_atomic_head_step {p E Φ} e1 :
-  to_val e1 = None →
-  (∀ σ1, state_interp σ1 ={E}=∗
-    ⌜if p then head_reducible e1 σ1 else True⌝ ∗
-    ▷ ∀ e2 σ2 efs, ⌜prim_step e1 σ1 e2 σ2 efs⌝ ={E}=∗
-      state_interp σ2 ∗ default False (to_val e2) Φ
-      ∗ [∗ list] ef ∈ efs, WP ef @ p; ⊤ {{ _, True }})
+      default False (to_val e2) Φ ∗ [∗ list] ef ∈ efs, WP ef @ p; ⊤ {{ _, True }})
   ⊢ WP e1 @ p; E {{ Φ }}.
 Proof.
   iIntros (?) "H". iApply wp_lift_atomic_step; eauto.
-  iIntros (σ1) "Hσ1". iMod ("H" $! σ1 with "Hσ1") as "[% H]"; iModIntro.
-  iSplit; first by destruct p; eauto.
-  by iNext; iIntros (e2 σ2 efs ?); iApply "H"; eauto.
+  iIntros (σ1) "Hσ1". iMod ("H" with "Hσ1") as "[% H]"; iModIntro.
+  iSplit; first by destruct p; auto. iNext. iIntros (e2 σ2 efs) "%".
+  iApply "H"; auto.
 Qed.
 
-Lemma wp_lift_atomic_head_step_no_fork {E Φ} e1 :
+Lemma wp_lift_atomic_head_step_no_fork {p E Φ} e1 :
   to_val e1 = None →
   (∀ σ1, state_interp σ1 ={E}=∗
     ⌜head_reducible e1 σ1⌝ ∗
     ▷ ∀ e2 σ2 efs, ⌜head_step e1 σ1 e2 σ2 efs⌝ ={E}=∗
       ⌜efs = []⌝ ∗ state_interp σ2 ∗ default False (to_val e2) Φ)
-  ⊢ WP e1 @ E {{ Φ }}.
+  ⊢ WP e1 @ p; E {{ Φ }}.
 Proof.
   iIntros (?) "H". iApply wp_lift_atomic_head_step; eauto.
   iIntros (σ1) "Hσ1". iMod ("H" $! σ1 with "Hσ1") as "[$ H]"; iModIntro.
   iNext; iIntros (v2 σ2 efs) "%".
   iMod ("H" $! v2 σ2 efs with "[# //]") as "(% & $ & $)"; subst; auto.
-Qed.
-
-(* PDS: Discard. *)
-Lemma wp_strong_lift_atomic_head_step_no_fork {p E Φ} e1 :
-  to_val e1 = None →
-  (∀ σ1, state_interp σ1 ={E}=∗
-    ⌜if p then head_reducible e1 σ1 else True⌝ ∗
-    ▷ ∀ e2 σ2 efs, ⌜prim_step e1 σ1 e2 σ2 efs⌝ ={E}=∗
-      ⌜efs = []⌝ ∗ state_interp σ2 ∗ default False (to_val e2) Φ)
-  ⊢ WP e1 @ p; E {{ Φ }}.
-Proof.
-  iIntros (?) "H". iApply wp_strong_lift_atomic_head_step; eauto.
-  iIntros (σ1) "Hσ1". iMod ("H" with "Hσ1") as "[$ H]"; iModIntro.
-  iNext; iIntros (v2 σ2 efs) "%".
-  iMod ("H" with "[#]") as "(% & $ & $)"=>//; subst.
-  by iApply big_sepL_nil.
 Qed.
 
 Lemma wp_lift_pure_det_head_step {p E E' Φ} e1 e2 efs :
@@ -183,19 +110,6 @@ Lemma wp_lift_pure_det_head_step {p E E' Φ} e1 e2 efs :
 Proof using Hinh.
   intros. rewrite -(wp_lift_pure_det_step e1 e2 efs); eauto.
   destruct p; by auto.
-Qed.
-
-(* PDS: Discard. *)
-Lemma wp_strong_lift_pure_det_head_step {p E Φ} e1 e2 efs :
-  to_val e1 = None →
-  (∀ σ1, if p then head_reducible e1 σ1 else True) →
-  (∀ σ1 e2' σ2 efs',
-    prim_step e1 σ1 e2' σ2 efs' → σ1 = σ2 ∧ e2 = e2' ∧ efs = efs') →
-  ▷ (WP e2 @ p; E {{ Φ }} ∗ [∗ list] ef ∈ efs, WP ef @ p; ⊤ {{ _, True }})
-  ⊢ WP e1 @ p; E {{ Φ }}.
-Proof using Hinh.
-  iIntros (???) "H"; iApply wp_lift_pure_det_step; eauto.
-  by destruct p; eauto.
 Qed.
 
 Lemma wp_lift_pure_det_head_step_no_fork {p E E' Φ} e1 e2 :
@@ -218,17 +132,5 @@ Lemma wp_lift_pure_det_head_step_no_fork' {p E Φ} e1 e2 :
 Proof using Hinh.
   intros. rewrite -[(WP e1 @ _ {{ _ }})%I]wp_lift_pure_det_head_step_no_fork //.
   rewrite -step_fupd_intro //.
-Qed.
-
-(* PDS: Discard. *)
-Lemma wp_strong_lift_pure_det_head_step_no_fork {p E Φ} e1 e2 :
-  to_val e1 = None →
-  (∀ σ1, if p then head_reducible e1 σ1 else True) →
-  (∀ σ1 e2' σ2 efs',
-    prim_step e1 σ1 e2' σ2 efs' → σ1 = σ2 ∧ e2 = e2' ∧ [] = efs') →
-  ▷ WP e2 @ p; E {{ Φ }} ⊢ WP e1 @ p; E {{ Φ }}.
-Proof using Hinh.
-  intros. rewrite -(wp_lift_pure_det_step e1 e2 []) ?big_sepL_nil ?right_id; eauto.
-  by destruct p; eauto.
 Qed.
 End wp.
